\documentclass[11pt, oneside]{article}
\usepackage[letterpaper, margin=2cm]{geometry}
\usepackage{MATH666}
\usepackage{booktabs}

\begin{document}
\noindent \textbf{\Large{Caleb Logemann \\
MATH666 Finite Element Methods \\
Homework 1
}}
\pagebreak

%\lstinputlisting[language=MATLAB]{H01_23.m}
\begin{enumerate}
  \item[\#1]
    \begin{enumerate}
    \item[(a)] % Done
      In order to recast this as a variational problem we will multiply the
      equation by a test function and integrate.

      \begin{align*}
        -u'' + q u &= f \\
        -\dintt{-\pi}{\pi}{u''v}{x} + \dintt{-\pi}{\pi}{quv}{x} &= \dintt{-\pi}{\pi}{fv}{x}\\
        \dintt{-\pi}{\pi}{u'v'}{x} - \eval*{\p{u'v}}{-\pi}{\pi}+ \dintt{-\pi}{\pi}{quv}{x} &= \dintt{-\pi}{\pi}{fv}{x} \\
        \intertext{If we let $v(\pi) = v(-\pi)$, then the boundary term goes to zero because $u'(\pi) = u'(-\pi)$}
        \dintt{-\pi}{\pi}{u'v'}{x} + \dintt{-\pi}{\pi}{quv}{x} &= \dintt{-\pi}{\pi}{fv}{x}
      \end{align*}
      Thus the variational problem is to find a $u \in V$ where
      \[
        V = \set{\dintt*{-\pi}{\pi}{(u')^2 + qu^2}{x} < \infty | u(\pi) = u(-\pi), u'(\pi) = u'(-\pi)}
      \]
      such that
      \begin{align*}
        \dintt{\pi}{\pi}{u'v'}{x} + \dintt{-\pi}{\pi}{quv}{x} &= \dintt{-\pi}{\pi}{fv}{x}
      \end{align*}
      for all $v \in V$.
      The test function $v$ must satisfy the periodic boundary conditions on the
      function value, but I believe we can also choose to have $v$ satisfy the
      periodic condition on the derivative as well.
      This makes the test and trial function spaces the same.

    \item[(b)] % Done
      The energy minimization problem that is equivalent to the variational
      problem is to find a $u \in V$ such that
      \[
        F(u) \le F(w)
      \]
      for all $w \in V$, where
      \[
        F(w) = \frac{1}{2}\p{\dintt{\pi}{\pi}{(w')^2}{x} + \dintt{-\pi}{\pi}{qw^2}{x}} - \dintt{-\pi}{\pi}{fw}{x}
      \]
      I will now prove that the energy minimization problem and the variational
      problem are equivalent.

      \begin{proof}
        Let $u$ be a solution to the variational problem, and consider some
        $w \in V$.
        Then there exists $v \in V$ such that $u + v = w$.
        Now consider $F(w)$.
        \begin{align*}
          F(w) &= F(u + v) \\
          &= \frac{1}{2}\p{\dintt{\pi}{\pi}{(u'+v')^2}{x} + \dintt{-\pi}{\pi}{q(u+v)^2}{x}} - \dintt{-\pi}{\pi}{f(u+v)}{x} \\
          &= \frac{1}{2}\p{\dintt{\pi}{\pi}{(u')^2+2u'v' + (v')^2}{x} + \dintt{-\pi}{\pi}{qu^2+2quv + qv^2}{x}} - \dintt{-\pi}{\pi}{f(u+v)}{x} \\
          &= \frac{1}{2}\dintt{\pi}{\pi}{(u')^2 + qu^2}{x} - \dintt{-\pi}{\pi}{fu}{x} + \dintt{-\pi}{\pi}{u'v' + quv}{x} - \dintt{-\pi}{\pi}{fv}{x} + \frac{1}{2}\dintt{-\pi}{\pi}{(v')^2 + qv^2}{x} \\
          &= F(u) + \dintt{-\pi}{\pi}{u'v'}{x} + \dintt{-\pi}{\pi}{quv}{x} - \dintt{-\pi}{\pi}{fv}{x} +  \dintt{-\pi}{\pi}{(v')^2 + qv^2}{x} \\
          \intertext{Since $u$ is a solution to the variational problem the middle three terms cancel}
          &= F(u) +  \dintt{-\pi}{\pi}{(v')^2 + qv^2}{x} \\
          \intertext{Also since $q(x) > 0$ for $x \in \br{-\pi, \pi}$, this integral is nonnegative}
          &\ge F(u)
        \end{align*}

        This shows that $u$ is a solution to the energy minimization problem when
        $u$ is a solution to the variational problem.

        Now let $u$ be a solution to the energy minimization problem, then 
        \[
          F(u) \le F(w)
        \]
        for all $w \in V$.
        Let $v \in V$ and consider $w = u + \varepsilon v$, then
        $F(u) \le F(u + \varepsilon v)$.
        Consider the function of $\varepsilon$,
        \[
          g(\varepsilon) = F(u + \varepsilon v)
        \]
        we know that $g$ has a minimum at $\varepsilon = 0$ thus $g'(0) = 0$.
        \begin{align*}
          g(\varepsilon) &= \frac{1}{2}\p{\dintt{\pi}{\pi}{(u'+\varepsilon v')^2}{x} + \dintt{-\pi}{\pi}{q(u+\varepsilon v)^2}{x}} - \dintt{-\pi}{\pi}{f(u+\varepsilon v)}{x} \\
          %&= \frac{1}{2}\p{\dintt{\pi}{\pi}{(u')^2}{x} + \dintt{-\pi}{\pi}{qu^2}{x}} - \dintt{-\pi}{\pi}{fu}{x} + \varepsilon\dintt{-\pi}{\pi}{u'v'}{x} + \varepsilon\dintt{-\pi}{\pi}{quv}{x} - \varepsilon\dintt{-\pi}{\pi}{fv}{x} + \varepsilon^2\dintt{-\pi}{\pi}{(v')^2 + qv^2}{x} \\
          g'(\varepsilon) &= \dintt{-\pi}{\pi}{u'v'}{x} + \dintt{-\pi}{\pi}{quv}{x} - \dintt{-\pi}{\pi}{fv}{x} + 2\varepsilon\dintt{-\pi}{\pi}{(v')^2 + qv^2}{x} \\
          g'(0) &= \dintt{-\pi}{\pi}{u'v'}{x} + \dintt{-\pi}{\pi}{quv}{x} - \dintt{-\pi}{\pi}{fv}{x} \\
          0 &= \dintt{-\pi}{\pi}{u'v'}{x} + \dintt{-\pi}{\pi}{quv}{x} - \dintt{-\pi}{\pi}{fv}{x} \\
          \dintt{-\pi}{\pi}{fv}{x} &= \dintt{-\pi}{\pi}{u'v'}{x} + \dintt{-\pi}{\pi}{quv}{x} \\
        \end{align*}
        Since this is true for any $v \in V$, this shows that $u$ is a solution
        to the variational problem.
      \end{proof}

    \item[(c)] % Done
      Consider $u, w \in V$ solutions to the variational, then for any $v \in V$
      we have
      \begin{align*}
        \dintt{\pi}{\pi}{u'v'}{x} + \dintt{-\pi}{\pi}{quv}{x} &= \dintt{-\pi}{\pi}{fv}{x} \\
        \dintt{\pi}{\pi}{w'v'}{x} + \dintt{-\pi}{\pi}{qwv}{x} &= \dintt{-\pi}{\pi}{fv}{x} \\
        \dintt{\pi}{\pi}{(u - w)'v'}{x} + \dintt{-\pi}{\pi}{q(u - w)v}{x} &= 0
      \end{align*}
      Thus the Galerkin Orthogonality property of this problem is
      \[
        \dintt{\pi}{\pi}{(u - w)'v'}{x} + \dintt{-\pi}{\pi}{q(u - w)v}{x} = 0
      \]
      for $u$, $w$ solutions to the variational problem and for all $v \in V$.

      The energy norm for this problem is found by letting $v = u - w$ and
      taking the squareroot.
      \[
        \norm[E]{u} = \sqrt{\dintt{\pi}{\pi}{(u')^2}{x} + \dintt{-\pi}{\pi}{qu^2}{x}}
      \]

      Note that an energy inner product can be formed as well,
      \[
        \br[E]{u, v} = \dintt{\pi}{\pi}{u'v'}{x} + \dintt{-\pi}{\pi}{quv}{x}
        \qquad \norm[E]{u} = \sqrt{\br[E]{u, u}}
      \]
      This satisfies all the properties of an inner product.
      \begin{align*}
        \br[E]{u, v} &= \br[E]{v, u} \\
        \br[E]{au, v} &= a\br[E]{u, v} \\
        \br[E]{u + w, v} &= \br[E]{u, v} + \br[E]{w, v} \\
        \br[E]{u, u} \ge 0 \\
        \br[E]{u, u} = 0 &\Leftrightarrow u = 0
      \end{align*}
      Note that $q > 0$ is required for the last two statements.
      The fact that this forms an inner product allows the Cauchy-Schwarz
      inequality to be applied directly to the energy norm.
      Also the Galerkin Orthogonality condition can be expressed as
      \[
        \br[E]{u - w, v} = 0
      \]
      for $u, w$ solutions to the variational problem and for all $v \in V$.

    \item[(d)] % Done
      The cG(1) method for this problem is formulated by replacing the test and
      trial space $V$ with a subspace, $V^1_h$.
      Let $-\pi = x_0 < x_1 < \cdots < x_M < x_{M+1} = \pi$ be a partition of
      $\br{-\pi, \pi}$, and define $h_j = x_{j} - x_{j-1}$ and let
      $h = \max[1 \le j \le M+1]{h_j}$.
      I will also define the functions
      \[
        \phi_j(x) =
        \begin{cases}
          \frac{x - x_{j-1}}{x_j - x_{j-1}} & x_{j-1} \le x \le x_j \\
          \frac{x - x_{j+1}}{x_j - x_{j+1}} & x_{j} \le x \le x_{j+1} \\
          0 & \text{otherwise}
        \end{cases}
      \]
      for $j = 1, 2, \cdots, M$ and
      \[
        \phi_0(x) = \phi_{M+1}(x) =
        \begin{cases}
          \frac{x - x_{0}}{x_1 - x_0} & x_{0} \le x \le x_1 \\
          \frac{x - x_{M+1}}{x_M - x_{M+1}} & x_M \le x \le x_{M+1} \\
          0 & \text{otherwise}
        \end{cases}
      \]

      Then the space $V^1_h = \set{\sum{j = 1}{M+1}{\xi_j \phi_j} | \xi_{M+1} = \frac{h_1 h_{M+1}}{h_1 + h_{M+1}}\p{\frac{\xi_1}{h_1} + \frac{\xi_M}{h_{M+1}}}}$.
      The condition on $\xi_{M+1}$ guarantees the continuity of the derivative
      at $x_0 = x_{M+1}$.
      The design of the basis function $\phi_{M+1}$ guarantees the continuity of
      the function.

    \item[(e)] % Done
      The following will show that the cG(1) method gives the optimal solution
      in the energy norm.

      \begin{proof}
        Let $u$ be the solution to the original variational and let $U$ be the
        solution to the cG(1) method.
        Consider an arbitrary $v \in V^1_h$, and note that Galerkin orthogonality states
        that $\br[E]{u - U, U - v} = 0$.
        \begin{align*}
          \norm[E]{u - U}^2 &= \br[E]{u - U, u - U} \\
          &= \br[E]{u - U, u - U} + \br[E]{u - U, U - v} \\
          &= \br[E]{u - U, u - v}
          \intertext{Using Cauchy-Schwarz}
          &\le \norm[E]{u - U}\norm[E]{u - v}
        \end{align*}
        This shows that $\norm[E]{u - U} \le \norm[E]{u - v}$.
      \end{proof}

      Now in order to find an error estimate let $v = \pi_h u$.
      \begin{align*}
        \norm[E]{u - U}^2 &\le \norm[E]{u - \pi_h u}^2 \\
        &= \dintt{-\pi}{\pi}{((u - \pi_h u)')^2}{x} + \dintt{-\pi}{\pi}{q(u - \pi_h u)^2}{x} \\
        &\le C h^2 \norm{u''}^2 + C h^4 \norm{u''}^2
      \end{align*}
      Thus
      \[
        \norm[E]{u - U} \le C h \norm{u''}
      \]
      since the $h$ term dominates the error.

    \item[(f)] % Done
      Now I will find an error estimate in the $L^2$ norm.

      First note that this problem is self adjoint, and so the dual problem is
      \begin{align*}
        -\phi'' + q \phi &= e \\
        \phi(-\pi) &= \phi(\pi) \\
        \phi'(-\pi) &= \phi'(\pi) \\
      \end{align*}

      Now consider $\norm[L^2]{e}^2$,
      \begin{align*}
        \norm[L^2]{e}^2 &= \dintt{-\pi}{\pi}{e^2}{x}
        \intertext{Using the dual problem}
        &= \dintt{-\pi}{\pi}{e\p{-\phi'' + q\phi}}{x} \\
        &= -\dintt{-\pi}{\pi}{e\phi''}{x} + \dintt{-\pi}{\pi}{qe\phi}{x} \\
        &= \dintt{-\pi}{\pi}{e'\phi'}{x} + \dintt{-\pi}{\pi}{qe\phi}{x}
        \intertext{Using Galerkin Orthogonality}
        &= \dintt{-\pi}{\pi}{e'\phi'}{x} + \dintt{-\pi}{\pi}{qe\phi}{x} - \dintt{-\pi}{\pi}{e'\pi_h\phi'}{x} - \dintt{-\pi}{\pi}{qe\pi_h\phi}{x} \\
        &= \dintt{-\pi}{\pi}{e'(\phi - \pi_h \phi)'}{x} + \dintt{-\pi}{\pi}{qe(\phi - \pi_h\phi)}{x} \\
        &= \br[E]{e, \phi - \pi_h \phi}
        \intertext{Now applying Cauchy-Schwarz}
        &\le \norm[E]{e} \norm[E]{\phi - \pi_h \phi}
        \intertext{From part (e)}
        &\le C h \norm{u''} \norm[E]{\phi - \pi_h \phi}
      \end{align*}
      Now consider $\norm[E]{\phi - \pi_h \phi}$
      \begin{align*}
        \norm[E]{\phi - \pi_h \phi}^2 &= \dintt{-\pi}{\pi}{((\phi - \pi_h \phi)')^2}{x} + \dintt{-\pi}{\pi}{q(\phi - \pi_h \phi)^2}{x} \\
        &\le C_1 h^2 \norm{\phi''}^2 + C_2 h^4 \norm{\phi''}^2
        \intertext{Since the $h^2$ term dominates, the $h^4$ term can be incorporated into $C_1$}
        &\le C_1 h^2 \norm{\phi''}^2
      \end{align*}
      Therefore $\norm[E]{\phi - \pi_h \phi} \le C h \norm{\phi''}$.

      Next I will show that $\norm{\phi''} \le C \norm{e}$.
      Consider the dual problem again.
      \begin{align*}
        -\phi'' + q\phi &= e \\
        \dintt{-\pi}{\pi}{(-\phi'' + q\phi)^2}{x} &= \dintt{-\pi}{\pi}{e^2}{x} \\
        \dintt{-\pi}{\pi}{(\phi'')^2 - 2q\phi''\phi + q^2\phi^2}{x} &= \dintt{-\pi}{\pi}{e^2}{x} \\
        \norm{\phi''}^2 + \dintt{-\pi}{\pi}{-2q\phi''\phi + q^2\phi^2}{x} &= \norm{e}^2\\
        \norm{\phi''}^2 + \dintt{-\pi}{\pi}{2q(\phi')^2 + q^2\phi^2}{x} &= \norm{e}^2\\
        \norm{\phi''}^2 &= \norm{e}^2 - \dintt{-\pi}{\pi}{2q(\phi')^2 + q^2\phi^2}{x}\\
        \intertext{Since $\dintt{-\pi}{\pi}{2q(\phi')^2 + q^2\phi^2}{x}$ is strictly positive}
        \norm{\phi''}^2 &\le \norm{e}^2 \\
      \end{align*}
      Now putting this all together shows that 
      \[
        \norm[L^2]{e}^2 \le C h \norm[L^2]{u''} \norm[E]{\phi - \pi_h \phi} \le C h^2 \norm[L^2]{u''} \norm[L^2]{\phi''} \le C h^2 \norm[L^2]{u''} \norm[L^2]{e}
      \]
      Dividing both side by $\norm[L^2]{e}$ gives
      \[
        \norm[L^2]{e} \le C h^2 \norm[L^2]{u''}
      \]

    \item[(g)]
      The following function solves the cG(1) FEM.
      \lstinputlisting[language=MATLAB]{cg1.m}
      The following script uses this function to solve the given problem.
      \lstinputlisting[language=MATLAB, lastline=54]{HW1.m}

      The following table gives the rates of convergence.
      \begin{center}
        \begin{tabular}{cccccc}
          \toprule
          M+1 & h & Energy Error & Energy Order & L2 Error & L2 Order \\
          \midrule
           10 & .628 & 1.02 & - & 0.17   & -\\
           20 & .314 & 0.52 & 1 & 0.04   & 2\\
           40 & .157 & 0.26 & 1 & 0.01   & 2\\
           80 & .078 & 0.13 & 1 & 0.0026 & 2\\
          160 & .039 & 0.65 & 1 & 0.0007 & 2\\
          \bottomrule
        \end{tabular}
      \end{center}

    \end{enumerate}

  \item[\#2]
    \begin{enumerate}
      \item[(a)] % Done
        In order to recast this as a variational problem I will multiply by a
        test function and integrate.

        \begin{align*}
          u^{(iv)} &= f \\
          \dintt{0}{1}{u^{(iv)}v}{x} &= \dintt{0}{1}{fv}{x} \\
          -\dintt{0}{1}{u'''v'}{x} + \eval*{u'''v}{x = 0}{1} &= \dintt{0}{1}{fv}{x} \\
          \dintt{0}{1}{u''v''}{x} - \eval*{u''v'}{x = 0}{1} + \eval*{u'''v}{x = 0}{1} &= \dintt{0}{1}{fv}{x} \\
          \intertext{Letting $v(0) = 0$ and $v'(0) = 0$ gives}
          \dintt{0}{1}{u''v''}{x} &= \dintt{0}{1}{fv}{x} \\
        \end{align*}
        Thus the Bilinear operator and Linear operator of this varational
        problem are
        \[
          B(u, v) = \dintt{0}{1}{u''v''}{x} \qquad L(v) = \dintt{0}{1}{fv}{x}
        \]
        The test and trial functions must be smooth enough to be well defined
        for these operators, so $u$ and $v$ must be in
        \[
          V = \set{\dintt{0}{1}{(u'')^2 + (u')^2 + u^2}{x} < \infty | u(0) = 0,
            u'(0) = 0, u''(1) = 0, u'''(1) = 0}
        \]
        The test functions must satisfy the same boundary conditions in order
        for this operator to be self-adjoint.

      \item[(b)] % Done
        The energy functional is given by
        \[
          F(w) = \frac{1}{2}B(w, w) - L(w) = \frac{1}{2}\dintt{0}{1}{(w'')^2}{x} - \dintt{0}{1}{fw}{x}
        \]
        Therefore the energy minimization problem is to find a $u \in V$ such that
        \[
          F(u) \le F(w)
        \]
        for all $w \in V$.
        Next I will prove that these two problems are equivalent.

        \begin{proof}
          Let $u$ be a solution to the Energy Minimization problem, and
          let $v \in V$.
          Now consider $g(\varepsilon) = F(u + \varepsilon v)$.
          Since $F$ has a minimum at $u$, this means that $g'(0) = 0$.
          \begin{align*}
            g(\varepsilon) &= \frac{1}{2}\dintt{0}{1}{((u + \varepsilon v)'')^2}{x} - \dintt{0}{1}{f(u + \varepsilon v)}{x} \\
            g'(\varepsilon) &= \dintt{0}{1}{((u + \varepsilon v)'')v''}{x} - \dintt{0}{1}{fv}{x} \\
            g'(0) &= \dintt{0}{1}{u''v''}{x} - \dintt{0}{1}{fv}{x} \\
            0 &= \dintt{0}{1}{u''v''}{x} - \dintt{0}{1}{fv}{x} \\
            \dintt{0}{1}{u''v''}{x} &= \dintt{0}{1}{fv}{x} \\
          \end{align*}
          Since this is true for any $v \in V$, $u$ is also a solution to the
          variational problem.

          Now let $u$ be a solution to the variational problem and let $w \in V$,
          then set $v = w - u$, so that $u + v = w$.
          \begin{align*}
            F(w) &= F(u + v) \\
            &= \frac{1}{2}\dintt{0}{1}{((u + v)'')^2}{x} - \dintt{0}{1}{f(u + v)}{x} \\
            &= \frac{1}{2}\dintt{0}{1}{(u'')^2 + 2u''v'' + (v'')^2}{x} - \dintt{0}{1}{f(u + v)}{x} \\
            &= \frac{1}{2}\dintt{0}{1}{(u'')^2}{x} - \dintt{0}{1}{fu}{x} + \dintt{0}{1}{u''v''}{x} - \dintt{0}{1}{fv}{x} + \frac{1}{2}\dintt{0}{1}{(v'')^2}{x} \\
            \intertext{Since $u$ is a solution to the variational problem}
            &= F(u) + \frac{1}{2}\dintt{0}{1}{(v'')^2}{x} \\
            &\ge F(u) \\
          \end{align*}
          Thus $u$ is also a solution to the Energy Minimization problem.
        \end{proof}

      \item[(c)] % Done
        The cG(3) method for this problem is formulated by replacing the test and
        trial space $V$ with a subspace, $V^3_h$.
        Let $-\pi = x_0 < x_1 < \cdots < x_M < x_{M+1} = \pi$ be a partition of
        $\br{-\pi, \pi}$, and define $h_j = x_{j} - x_{j-1}$ and let
        $h = \max[1 \le j \le M+1]{h_j}$.
        I will also define the functions
        \[
          \phi_j^1(x) =
          \begin{cases}
            \p{\frac{1}{h^2} - \frac{2(x - x_j)}{h^3}}\p{x - x_{j-1}}^2 & x_{j-1} \le x \le x_j \\
            \p{\frac{1}{h^2} + \frac{2(x - x_j)}{h^3}}\p{x - x_{j+1}}^2 & x_{j} \le x \le x_{j+1} \\
            0 & \text{otherwise}
          \end{cases}
        \]
        and
        \[
          \phi_j^2(x) =
          \begin{cases}
            (x - x_j)\frac{\p{x - x_{j-1}}^2}{h^2} & x_{j-1} \le x \le x_j \\
            (x - x_j)\frac{\p{x - x_{j+1}}^2}{h^2} & x_{j} \le x \le x_{j+1} \\
            0 & \text{otherwise}
          \end{cases}
        \]
        for $j = 1, 2, \cdots, M$ and
        \[
          \phi_{M+1}^1(x) =
          \begin{cases}
            \p{\frac{1}{h^2} - \frac{2(x - x_{M+1})}{h^3}}\p{x - x_{M}}^2 & x_{M} \le x \le x_{M+1} \\
            0 & \text{otherwise}
          \end{cases}
        \]
        \[
          \phi_{M+1}^2(x) =
          \begin{cases}
            (x - x_{M+1})\frac{\p{x - x_{M}}^2}{h^2} & x_{M} \le x \le x_{M+1} \\
            0 & \text{otherwise}
          \end{cases}
        \]
        for $j = M+1$.

        Then the space $V^3_h = \spanspace{\phi_j^1, \phi_j^2}_{j=1}^{M+1}$.
        The design of the basis functions guarantees the continuity of the
        function and its derivative.

        Thus the FEM is to find a solution to the variational problem in $V^3_h$,
        that is find $u \in V^3_h$ such that
        \[
          B(u, v) = L(v)
        \]
        for all $v \in V^3_h$.

      \item[(d)] % Done
        Next I will find a a priori estimate for the error in terms of the
        energy norm.
        \begin{align*}
          \norm[E]{e}^2 &= \norm[E]{u - u_h}^2 \\
          &= B(u - u_h, u - u_h)
          \intertext{By Galerkin Orthogonality $B(u - u_h, u_h - \pi_h u) = 0$, so}
          &= B(u - u_h, u - u_h) + B(u - u_h, u_h - \pi_h u) \\
          &= B(u - u_h, u - \pi_h u)
          \intertext{Using Cauchy-Schwarz}
          &\le \norm[E]{u - u_h} \norm[E]{u - \pi_h u} \\
          \norm[E]{e} &\le \norm[E]{u - \pi_h u} \\
          &\le \sqrt{\dintt{0}{1}{((u - \pi_h u)'')^2}{x}} \\
          &\le \sqrt{\dintt{0}{1}{(ch^2\norm[L^2]{u^{(iv)}})^2}{x}} \\
          &\le ch^2\norm[L^2]{u^{(iv)}} \\
        \end{align*}
        Thus this method is second order accurate in the energy norm.

      \item[(e)] % Done
        The error estimate in the $L^2$ norm can be found by considering the
        dual problem.
        Since this problem is self-adjoint, the dual problem is
        \begin{align*}
          \phi^{(iv)} = f \\
          \phi(0) = \phi'(0) = \phi''(1) = \phi'''(1) = 0
        \end{align*}

        Now consider $\norm[L^2]{e}^2$.
        \begin{align*}
          \norm[L^2]{e}^2 &= \dintt{0}{1}{e^2}{x} \\
          &= \dintt{0}{1}{e \phi^{(iv)}}{x} \\
          &= -\dintt{0}{1}{e' \phi'''}{x} \\
          &= \dintt{0}{1}{e'' \phi''}{x}
          \intertext{Using Galerkin Orthogonality}
          &= \dintt{0}{1}{e'' \phi''}{x} - \dintt{0}{1}{e''(\pi_h \phi)''}{x}\\
          &= \dintt{0}{1}{e'' (\phi - \pi_h \phi)''}{x}
          \intertext{By the Cauchy-Scwarz Inequality}
          &\le \norm[E]{e} \norm[E]{\phi - \pi_h \phi} \\
          &\le C h^2\norm[L^2]{u^{(iv)}} Ch^2 \norm[L^2]{\phi^{(iv)}}
          \intertext{Using the dual problem and taking the $L^2$ norm of both
          sides, we see that $\norm[L^2]{\phi^{(iv)}} = \norm[L^2]{e}$}.
          \norm[L^2]{e}^2 &\le C h^4 \norm[L^2]{u^{(iv)}} \norm[L^2]{e} \\
          \norm[L^2]{e} &\le C h^4 \norm[L^2]{u^{(iv)}} \\
        \end{align*}
        Thus the FEM is fourth order accurate in the $L^2$ norm.

      \item[(f)]
        The following function solves the cG(3) FEM.
        \lstinputlisting[language=MATLAB]{cg3.m}
        The following script uses this function to solve the given problem.
        \lstinputlisting[language=MATLAB, firstline=51, lastline=124]{HW1.m}

        The following shows the order of convergence
        \begin{center}
          \begin{tabular}{cccccc}
            \toprule
            M+1 & h & Energy Error & Energy Order & L2 Error & L2 Order \\
            \midrule
             10 & 0.1     & 3.6   & -    & 0.0016    & -\\
             20 & 0.05    & 0.9   & 1.99 & 0.0001    & 3.99\\
             40 & 0.025   & 0.22  & 1.99 & 0.000006  & 4.02\\
             80 & 0.0125  & 0.057 & 1.99 & 0.0000004 & 3.83\\
            160 & 0.00625 & 0.013 & 2.05 & 0.0000004 & 0.065\\
            \bottomrule
          \end{tabular}
        \end{center}
    \end{enumerate}

\end{enumerate}
\end{document}
