\documentclass[11pt, titlepage]{article}
\author{Caleb Logemann}
\title{MATH 666: Finite Element Methods \\ Homework 3}
\date{December 4, 2018}
\usepackage[letterpaper, margin=2cm]{geometry}
\usepackage{MATH666}
\usepackage{booktabs}

\begin{document}
\maketitle

%\lstinputlisting[language=MATLAB]{H01_23.m}
\begin{enumerate}
  \item[\#1]
    Consider the Crank-Nicolson-cG(1) FEM for the diffusion equation.
    Find $u^n_h \in V^1_h$ such that
    \begin{gather*}
      \abr{\frac{u^n_h - u^n_h}{\delta T}, v} + 
      \abr{\grad \frac{u_h^n + u_h^{n-1}}{2}, \grad v} = 
      \abr{\frac{f^n + f^{n-1}}{2}, v} 
      \quad \forall v \in V^1_h, n = 1, 2, 3, \ldots, \\
      \abr{u^0_h, v} = \abr{u_0, v}
    \end{gather*}
    Following the convergence proof of the Backward-Euler-cG(1) FEM from class,
    prove that the Crank-Nicolson-cG(1) FEM satisfies:
    \[
      \norm{u^n_h - u(t^n)} = \mcO\p{\Delta t^2 + h^2}.
    \]

    The initial variational problem is formulated as finding $u \in V$ such that
    \begin{gather*}
      \abr{u_t, v} + \abr{\grad u, \grad v} = \abr{f, v} \quad \forall v \in V \\
      \abr{u(0, x), v} = \abr{u_0, v}
    \end{gather*}
    The semidescrete form of the FEM can be expressed as finding $u_h \in V^1_h$
    such that
    \[
      \abr{\p{u_h}_t, v} + \abr{\grad u_h, \grad v} = \abr{f, v} \quad \forall v \in V^1_h
      \abr{u_h(0, x), v} = \abr{u_0, v}
    \]

    I will also make use of the following projection $R_h(u)$ which satisfies
    \[
      \abr{\grad R_h(u), \grad v} = \abr{\grad u, \grad v} \quad \forall v \in V^1_h
    \]

    Suppose $u$ is the solution to the original variational problem, then
    for all $v \in V^1_h$,
    \begin{align*}
      \abr{u_t, v} + \abr{\grad u, \grad v} &= \abr{f, v} \\
      \abr{u_t, v} + \abr{\grad R_h(u), \grad v} &= \abr{f, v} \\
    \end{align*}
    This is true for every time $t > 0$, in particular it is true at times
    $t^n$ and $t^{n-1}$, so
    \begin{align*}
      \abr{u^n_t, v} + \abr{\grad R_h(u^n), \grad v} &= \abr{f^n, v} \\
      \abr{u^{n-1}_t, v} + \abr{\grad R_h(u^{n-1}), \grad v} &= \abr{f^{n-1}, v} \\
      \abr{\frac{u^n_t + u^{n-1}_t}{2}, v} + \abr{\grad R_h\p{\frac{u^n + u^{n-1}}{2}}, \grad v} &= \abr{\frac{f^n + f^{n-1}}{2}, v} \\
      \abr{\grad R_h\p{\frac{u^n + u^{n-1}}{2}}, \grad v} &= \abr{\frac{f^n + f^{n-1}}{2}, v} - \abr{\frac{u^n_t + u^{n-1}_t}{2}, v}\\
    \end{align*}
    Consider $u^n_h$ and $u^{n-1}_h$, solutions to the FEM, they satisfy
    \[
      \abr{\frac{u^n_h - u^n_h}{\delta T}, v} + 
      \abr{\grad \frac{u_h^n + u_h^{n-1}}{2}, \grad v} = 
      \abr{\frac{f^n + f^{n-1}}{2}, v} 
    \]
    Let $\theta^n = R_h u^n - u^n_h$, then subtracting the last two equations
    gives
    \begin{align*}
      
    \end{align*}

\end{enumerate}
\end{document}
